added STORE commutativity

Isabelle/IMAP.thy
@@ -3,9 +3,9 @@ imports ORSet
 	
 begin
 	
-(* 'a is the set of all foldernames, 'b is the set of all messagenames  *)
+-- "Type defeinition: 'a is the set of all foldernames, 'b is the set of all messagenames"
 type_synonym ('a, 'b) imap = "'a orset \<times> ('a \<rightharpoonup> 'b set)"
-	
+
 abbreviation folderset ::
   "('a, 'b) imap \<Rightarrow> 'a orset" 
 where
@@ -15,14 +15,27 @@ abbreviation filesystem ::
   "('a, 'b) imap \<Rightarrow> ('a \<rightharpoonup> 'b set)"
 where
   "filesystem I \<equiv> snd I"
-  
-(*State Invariants*)
+
 definition validState ::
 	"('a,'b) imap \<Rightarrow> bool"
 	where
 	"validState I = ((\<forall> (a,_) \<in> folderset I . (filesystem I) a \<noteq> None)
 	\<and> (\<forall> f . (filesystem I) f \<noteq> None \<longrightarrow> (\<exists> (a,_) \<in> folderset I . a = f)))"
-  
+	
+definition replaceMsg ::
+	"'b \<Rightarrow> 'b \<Rightarrow> 'b set \<Rightarrow> 'b set"
+where
+	"replaceMsg msgold msgnew S = (S - {msgold}) \<union> {msgnew}"
+
+definition msgLookup ::
+  "'a \<Rightarrow> 'b \<Rightarrow> ('a, 'b) imap \<Rightarrow> bool"
+where
+  "msgLookup f msg I = (case (filesystem I)(f) of 
+			None \<Rightarrow> False | 
+			Some msgset \<Rightarrow> msg \<in> msgset)"
+
+-- "######### BEGIN OPERATIONS ##########"
+
 definition CREATE_atSource ::
 	"'a \<Rightarrow> ('a, 'b) imap \<Rightarrow> bool"
 where
@@ -32,13 +45,13 @@ definition CREATE_downstream ::
 	"'a \<Rightarrow> nat \<Rightarrow> ('a, 'b) imap \<Rightarrow> ('a, 'b) imap"
 where
 	"CREATE_downstream f n I = (add f n (folderset I), (filesystem I)(f := Some {}))"
-	
-(*computes the R set for a mailbox*)
+
 definition DELETE_atSource ::
 	"'a \<Rightarrow> ('a, 'b) imap \<Rightarrow> 'a orset"
 	where
 	"DELETE_atSource e I = remove_atSource e (folderset I)"
-	
+
+-- "unused"
 definition DELETE_atSource_pre ::
 	"'a \<Rightarrow> ('a, 'b) imap \<Rightarrow> bool"
 	where
@@ -63,73 +76,25 @@ where
 			None \<Rightarrow> filesystem I | 
 			Some msgset \<Rightarrow> (filesystem I)(f := Some (msgset \<union> {m})))
 	)"
+	
+definition STORE_atSource ::
+  "'a \<Rightarrow> 'b \<Rightarrow> 'b \<Rightarrow> ('a, 'b) imap \<Rightarrow> bool"
+where
+  "STORE_atSource f msgold msgnew I = ((\<exists> (a,_) \<in> folderset I . a = f) \<and> msgLookup f msgold I \<and> \<not>(msgLookup f msgnew I))"
+	
+definition STORE_downstream ::
+  "'a \<Rightarrow> 'b \<Rightarrow> 'b \<Rightarrow> ('a, 'b) imap \<Rightarrow> ('a, 'b) imap"
+where
+  "STORE_downstream f msgold msgnew I = 
+	(folderset I, 
+		(case (filesystem I)(f) of 
+			None \<Rightarrow> filesystem I | 
+			Some msgset \<Rightarrow> (filesystem I)(f := Some (replaceMsg msgold msgnew msgset)))
+	)"
+	
+-- "########## END OPERATIONS ##########"
 
-(*rewrite filesystem with option type?*)
-  
-lemma commCREATE:
-fixes
-  I :: "('a,'b) imap" and
-  e1 :: "'a" and
-  e2 :: "'a" and
-  n1 :: nat and
-  n2 :: nat
-assumes
-	n1neqn2: "n1 \<noteq> n2"
-shows 
-	"CREATE_downstream e1 n1 (CREATE_downstream e2 n2 I) = CREATE_downstream e2 n2 (CREATE_downstream e1 n1 I)"
-proof -
-	show ?thesis unfolding CREATE_downstream_def using commAdd n1neqn2 by fastforce
-qed
-	
-lemma commDELETE:
-fixes
-  I :: "('a, 'b) imap" and
-  R1 :: "'a orset" and
-  R2 :: "'a orset" and
-  e1 :: "'a" and
-  e2 :: "'a"
-assumes 
-  O1R1: " R1 = DELETE_atSource e1 I" and
-  O2R2: " R2 = DELETE_atSource e2 I"
-shows "DELETE_downstream e2 R2 (DELETE_downstream e1 R1 I) = DELETE_downstream e1 R1 (DELETE_downstream e2 R2 I)"
-proof -
-	show ?thesis using O1R1 O2R2 commRemove unfolding DELETE_downstream_def DELETE_atSource_def remove_atSource_def apply simp
-	proof -
-		assume a1: "R1 = {(a, b). (a, b) \<in> folderset I \<and> a = e1}"
-		assume a2: "R2 = {(a, b). (a, b) \<in> folderset I \<and> a = e2}"
-		have f3: "\<forall>P a Pa Pb aa. (P \<noteq> remove_atSource (a::'a) Pa \<or> Pb \<noteq> remove_atSource aa Pa) \<or> remove_downstream Pb (remove_downstream P Pa) = remove_downstream P (remove_downstream Pb Pa)"
-			by (meson commRemove)
-		have f4: "{(a, n). (a, n) \<in> folderset I \<and> a = e1} = remove_atSource e1 (folderset I)"
-			using a1 by (simp add: DELETE_atSource_def O1R1)
-		have "{(a, n). (a, n) \<in> folderset I \<and> a = e2} = remove_atSource e2 (folderset I)"
-			using a2 by (simp add: DELETE_atSource_def O2R2)
-		then show "remove_downstream {(a, n). (a, n) \<in> folderset I \<and> a = e2} (remove_downstream {(a, n). (a, n) \<in> folderset I \<and> a = e1} (folderset I)) = remove_downstream {(a, n). (a, n) \<in> folderset I \<and> a = e1} (remove_downstream {(a, n). (a, n) \<in> folderset I \<and> a = e2} (folderset I)) \<and> (filesystem I)(e1 := None, e2 := None) = (filesystem I) (e2 := None, e1 := None)"
-			using f4 f3 by auto
-	qed
-qed
-	
-lemma commCREATE_DELETE:
-fixes
-  I :: "('a, 'b) imap" and
-  R1 :: "'a orset" and
-  e1 :: "'a" and
-  e2 :: "'a" and
-  n :: nat
-assumes 
-  O1R1: " R1 = DELETE_atSource e1 I" and
-	freshn: "fresh n (folderset I)" and
-	O2pre: "CREATE_atSource e2 I" and
-	lookupe1: "lookup e1 (folderset I)"
-shows "DELETE_downstream e1 R1 (CREATE_downstream e2 n I) = CREATE_downstream e2 n (DELETE_downstream e1 R1 I)"
-proof -
-	have fset: "folderset (DELETE_downstream e1 R1 (CREATE_downstream e2 n I)) = folderset (CREATE_downstream e2 n (DELETE_downstream e1 R1 I))"
-		using O1R1 freshn unfolding DELETE_downstream_def CREATE_downstream_def fresh_def commAddRemove 
-		  DELETE_atSource_def remove_atSource_def remove_downstream_def add_def by auto		  
-	have "filesystem (DELETE_downstream e1 R1 (CREATE_downstream e2 n I)) = filesystem (CREATE_downstream e2 n (DELETE_downstream e1 R1 I))" 
-	  using O1R1 O2pre lookupe1 unfolding DELETE_downstream_def CREATE_downstream_def DELETE_atSource_def remove_atSource_def CREATE_atSource_def validState_def
-		lookup_def by fastforce
-	thus ?thesis using fset unfolding DELETE_downstream_def by auto
-qed
+-- "####### BEGIN HELPING LEMMAS #######"
 
 lemma append_not_none:
 fixes
@@ -166,7 +131,44 @@ assumes
 	validS: "validState I"
 shows "\<forall> f . f \<noteq> f1 \<longrightarrow> filesystem (APPEND_downstream f1 m1 I) f = filesystem I f"
 proof (simp add: APPEND_downstream_def option.case_eq_if)
-qed	
+qed
+
+lemma store_folderset:
+fixes
+  I :: "('a, 'b) imap" and
+  f :: "'a"
+shows "folderset (STORE_downstream f msgold msgnew I) = folderset I"
+proof -
+	show ?thesis unfolding STORE_downstream_def by auto
+qed
+
+lemma store_filesystem:
+fixes
+  I :: "('a, 'b) imap" and
+  f1 :: "'a"
+shows "\<forall> f. f \<noteq> f1 \<longrightarrow> filesystem (STORE_downstream f1 msgold msgnew I) f = filesystem I f"
+proof -
+	show ?thesis unfolding STORE_downstream_def by (simp add: option.case_eq_if)
+qed
+  
+lemma store_not_none:
+fixes
+  I :: "('a, 'b) imap" and
+  f1 :: "'a" and
+  msgold :: "'b" and
+  msgnew :: "'b"
+assumes
+  pre: "STORE_atSource f1 msgold msgnew I"
+shows "filesystem (STORE_downstream f1 msgold msgnew I) f1 \<noteq> None"
+proof -
+	show ?thesis using pre unfolding STORE_downstream_def STORE_atSource_def msgLookup_def
+	  by (metis fun_upd_same option.case_eq_if option.simps(3) snd_conv)
+qed
+
+
+-- "######## END HELPING LEMMAS ########"
+
+-- "###### BEGIN VALIDITY LEMMAS #######"
 
 lemma append_valid:
 fixes
@@ -217,7 +219,66 @@ proof -
   show ?thesis using validS unfolding CREATE_downstream_def add_def validState_def CREATE_atSource_def apply simp 
     by (simp add: split_def)
 qed
+  
+lemma store_valid:
+fixes
+  I :: "('a, 'b) imap" and
+  f :: "'a" and
+  msgold :: "'b" and
+  msgnew :: "'b"
+assumes
+	validS: "validState I"
+shows "validState (STORE_downstream f msgold msgnew I)"
+proof -
+  show ?thesis sorry
+qed
 
+-- "####### END VALIDITY LEMMAS ########"  
+
+-- "####### BEGIN COMMUTATIVITY ########"  
+
+lemma commCREATE:
+fixes
+  I :: "('a,'b) imap" and
+  e1 :: "'a" and
+  e2 :: "'a" and
+  n1 :: nat and
+  n2 :: nat
+assumes
+	n1neqn2: "n1 \<noteq> n2"
+shows 
+	"CREATE_downstream e1 n1 (CREATE_downstream e2 n2 I) = CREATE_downstream e2 n2 (CREATE_downstream e1 n1 I)"
+proof -
+	show ?thesis unfolding CREATE_downstream_def using commAdd n1neqn2 by fastforce
+qed
+	
+lemma commDELETE:
+fixes
+  I :: "('a, 'b) imap" and
+  R1 :: "'a orset" and
+  R2 :: "'a orset" and
+  e1 :: "'a" and
+  e2 :: "'a"
+assumes 
+  O1R1: " R1 = DELETE_atSource e1 I" and
+  O2R2: " R2 = DELETE_atSource e2 I"
+shows "DELETE_downstream e2 R2 (DELETE_downstream e1 R1 I) = DELETE_downstream e1 R1 (DELETE_downstream e2 R2 I)"
+proof -
+	show ?thesis using O1R1 O2R2 commRemove unfolding DELETE_downstream_def DELETE_atSource_def remove_atSource_def apply simp
+	proof -
+		assume a1: "R1 = {(a, b). (a, b) \<in> folderset I \<and> a = e1}"
+		assume a2: "R2 = {(a, b). (a, b) \<in> folderset I \<and> a = e2}"
+		have f3: "\<forall>P a Pa Pb aa. (P \<noteq> remove_atSource (a::'a) Pa \<or> Pb \<noteq> remove_atSource aa Pa) \<or> remove_downstream Pb (remove_downstream P Pa) = remove_downstream P (remove_downstream Pb Pa)"
+			by (meson commRemove)
+		have f4: "{(a, n). (a, n) \<in> folderset I \<and> a = e1} = remove_atSource e1 (folderset I)"
+			using a1 by (simp add: DELETE_atSource_def O1R1)
+		have "{(a, n). (a, n) \<in> folderset I \<and> a = e2} = remove_atSource e2 (folderset I)"
+			using a2 by (simp add: DELETE_atSource_def O2R2)
+		then show "remove_downstream {(a, n). (a, n) \<in> folderset I \<and> a = e2} (remove_downstream {(a, n). (a, n) \<in> folderset I \<and> a = e1} (folderset I)) = remove_downstream {(a, n). (a, n) \<in> folderset I \<and> a = e1} (remove_downstream {(a, n). (a, n) \<in> folderset I \<and> a = e2} (folderset I)) \<and> (filesystem I)(e1 := None, e2 := None) = (filesystem I) (e2 := None, e1 := None)"
+			using f4 f3 by auto
+	qed
+qed
+  
 lemma commAPPEND:
 fixes
   I :: "('a, 'b) imap" and
@@ -241,6 +302,93 @@ proof -
 	thus ?thesis using A1	by (simp add: prod_eq_iff)
 qed
   
+lemma commSTORE:
+fixes
+  I :: "('a, 'b) imap" and
+  f1 :: "'a" and
+  f2 :: "'a" and
+  mo1 :: "'b" and
+  mo2 :: "'b" and
+  mn1 :: "'b" and
+  mn2 :: "'b"
+assumes 
+  O1pre: " STORE_atSource f1 mo1 mn1 I" and
+  O2pre: " STORE_atSource f2 mo2 mn2 I" 
+shows "STORE_downstream f1 mo1 mn1 (STORE_downstream f2 mo2 mn2 I) = STORE_downstream f2 mo2 mn2 (STORE_downstream f1 mo1 mn1 I)"
+proof -
+  have A1: "folderset (STORE_downstream f1 mo1 mn1 (STORE_downstream f2 mo2 mn2 I)) = folderset(STORE_downstream f2 mo2 mn2 (STORE_downstream f1 mo1 mn1 I))"
+    by (simp add: store_folderset)
+  
+  have  A5: "\<forall> f . f1 \<noteq> f2 \<longrightarrow> filesystem (STORE_downstream f1 mo1 mn1 (STORE_downstream f2 mo2 mn2 I)) f = filesystem(STORE_downstream f2 mo2 mn2 (STORE_downstream f1 mo1 mn1 I)) f"
+    by (smt STORE_downstream_def fun_upd_twist option.case_eq_if snd_conv store_filesystem)
+    
+  have  "f1 = f2 \<longrightarrow> filesystem (STORE_downstream f1 mo1 mn1 (STORE_downstream f2 mo2 mn2 I)) f1 = filesystem(STORE_downstream f2 mo2 mn2 (STORE_downstream f1 mo1 mn1 I)) f1"
+  proof auto
+    assume Ass: "f1 = f2"
+    hence  "filesystem (STORE_downstream f1 mo1 mn1 (STORE_downstream f2 mo2 mn2 I)) f1 \<noteq> None"
+      by (smt O2pre STORE_downstream_def fun_upd_eqD fun_upd_triv option.case_eq_if option.simps(3) snd_conv store_not_none)
+  
+    hence "\<exists> y . filesystem (STORE_downstream f1 mo1 mn1 (STORE_downstream f2 mo2 mn2 I)) f1 = Some y"
+      by simp
+    
+    then obtain y where Ass4: "filesystem (STORE_downstream f1 mo1 mn1 (STORE_downstream f2 mo2 mn2 I)) f1 = Some y" by blast
+    
+    have "\<exists> S . filesystem (I) f1 = Some S" by (metis O2pre STORE_atSource_def \<open>f1 = f2\<close> case_optionE msgLookup_def)
+    then obtain S where Ass2: "(filesystem I) f1 = Some S" by blast
+        
+    have "\<exists> x . filesystem (STORE_downstream f2 mo2 mn2 I) f1 = Some x" using Ass by (metis O2pre option.collapse store_not_none) 
+    then obtain x where Ass3: "filesystem (STORE_downstream f2 mo2 mn2 I) f1 = Some x" by blast
+        
+    have "x = (S - {mo2}) \<union> {mn2}" using Ass Ass2 Ass3 unfolding STORE_downstream_def replaceMsg_def  by simp    
+        
+    hence Ass6: "y = (S - {mo1,mo2}) \<union> {mn1,mn2}" using Ass Ass2 Ass3 Ass4 O1pre O2pre unfolding STORE_downstream_def replaceMsg_def STORE_atSource_def
+      by auto
+        
+    have "\<exists> w . filesystem (STORE_downstream f1 mo1 mn1 I) f1 = Some w" using Ass by (metis O1pre option.collapse store_not_none)
+    then obtain w where Ass8: "filesystem (STORE_downstream f1 mo1 mn1 I) f1 = Some w" by blast
+        
+    hence Ass9: "w = (S - {mo1}) \<union> {mn1}" using Ass Ass2 unfolding STORE_downstream_def replaceMsg_def by simp
+        
+    have "filesystem(STORE_downstream f2 mo2 mn2 (STORE_downstream f1 mo1 mn1 I)) f1 \<noteq> None" using O1pre 
+        unfolding STORE_downstream_def using Ass Ass2 by auto
+      
+    hence "\<exists> z . filesystem(STORE_downstream f2 mo2 mn2 (STORE_downstream f1 mo1 mn1 I)) f1 = Some z"
+      by simp
+      
+    then obtain z where Ass7: "filesystem(STORE_downstream f2 mo2 mn2 (STORE_downstream f1 mo1 mn1 I)) f1 = Some z" by blast
+        
+    hence "z = (S - {mo1,mo2}) \<union> {mn1,mn2}" using Ass Ass2 Ass9 Ass8 O1pre O2pre unfolding STORE_downstream_def replaceMsg_def STORE_atSource_def by auto
+    
+    thus "filesystem (STORE_downstream f2 mo1 mn1 (STORE_downstream f2 mo2 mn2 I)) f2 =
+    filesystem (STORE_downstream f2 mo2 mn2 (STORE_downstream f2 mo1 mn1 I)) f2" using Ass7 Ass4 Ass6 Ass by auto
+  qed
+  thus ?thesis using A1 A5
+    by (smt O1pre O2pre STORE_downstream_def fun_upd_same fun_upd_twist fun_upd_upd option.case_eq_if prod_eqI snd_conv store_not_none)
+qed
+	
+lemma commCREATE_DELETE:
+fixes
+  I :: "('a, 'b) imap" and
+  R1 :: "'a orset" and
+  e1 :: "'a" and
+  e2 :: "'a" and
+  n :: nat
+assumes 
+  O1R1: " R1 = DELETE_atSource e1 I" and
+	freshn: "fresh n (folderset I)" and
+	O2pre: "CREATE_atSource e2 I" and
+	lookupe1: "lookup e1 (folderset I)"
+shows "DELETE_downstream e1 R1 (CREATE_downstream e2 n I) = CREATE_downstream e2 n (DELETE_downstream e1 R1 I)"
+proof -
+	have fset: "folderset (DELETE_downstream e1 R1 (CREATE_downstream e2 n I)) = folderset (CREATE_downstream e2 n (DELETE_downstream e1 R1 I))"
+		using O1R1 freshn unfolding DELETE_downstream_def CREATE_downstream_def fresh_def commAddRemove 
+		  DELETE_atSource_def remove_atSource_def remove_downstream_def add_def by auto		  
+	have "filesystem (DELETE_downstream e1 R1 (CREATE_downstream e2 n I)) = filesystem (CREATE_downstream e2 n (DELETE_downstream e1 R1 I))" 
+	  using O1R1 O2pre lookupe1 unfolding DELETE_downstream_def CREATE_downstream_def DELETE_atSource_def remove_atSource_def CREATE_atSource_def validState_def
+		lookup_def by fastforce
+	thus ?thesis using fset unfolding DELETE_downstream_def by auto
+qed
+  
 lemma commCREATE_APPEND:
 fixes
   I :: "('a, 'b) imap" and
@@ -259,6 +407,29 @@ proof -
     by (smt case_prodE fun_upd_apply fun_upd_twist option.case_eq_if prod.sel(2))
 	thus ?thesis using append_folderset[of f m I] unfolding APPEND_downstream_def CREATE_downstream_def by auto
 qed
+  
+lemma commDELETE_APPEND:
+fixes
+  I :: "('a, 'b) imap" and
+  f :: "'a" and
+  e :: "'a" and
+  m :: "'b" and
+  R :: "'a orset"
+assumes 
+  O1pre: " APPEND_atSource f m I" and
+  O2pre: " R = DELETE_atSource e I" and
+	validS: "validState I"
+shows "APPEND_downstream f m (DELETE_downstream e R I) = DELETE_downstream e R (APPEND_downstream f m I)"
+proof -
+  have A1: "folderset(APPEND_downstream f m (DELETE_downstream e R I)) = folderset(DELETE_downstream e R (APPEND_downstream f m I))"
+    unfolding DELETE_downstream_def by (simp add: append_folderset)
+  have "filesystem(APPEND_downstream f m (DELETE_downstream e R I)) = filesystem(DELETE_downstream e R (APPEND_downstream f m I))"
+    using O1pre O2pre unfolding APPEND_atSource_def APPEND_downstream_def DELETE_atSource_def DELETE_downstream_def 
+    by (simp add: fun_upd_twist option.case_eq_if)
+	thus ?thesis using A1 prod_eqI by blast
+qed
+  
+-- "######## END COMMUTATIVITY #########"  
   
 end
 	
